\documentclass{article}
\usepackage[utf8]{inputenc}
\usepackage{amsmath,amssymb,amsfonts,amsthm}
\usepackage{enumerate}

\begin{document}

% Working on part (a): Show dÎ± = 0

For the 1-form $\alpha = \frac{x dy - y dx}{x^2 + y^2}$ on $\mathbb{R}^2 \setminus \{0\}$.

We can write $\alpha = P dx + Q dy$ where:
- $P = \frac{-y}{x^2 + y^2}$
- $Q = \frac{x}{x^2 + y^2}$

To compute $d\alpha$:
$d\alpha = dP \wedge dx + dQ \wedge dy = \frac{\partial P}{\partial y} dy \wedge dx + \frac{\partial Q}{\partial x} dx \wedge dy$

Computing partial derivatives:
$\frac{\partial P}{\partial y} = \frac{\partial}{\partial y}\left(\frac{-y}{x^2 + y^2}\right) = \frac{-(x^2 + y^2) - (-y)(2y)}{(x^2 + y^2)^2} = \frac{-x^2 - y^2 + 2y^2}{(x^2 + y^2)^2} = \frac{y^2 - x^2}{(x^2 + y^2)^2}$

$\frac{\partial Q}{\partial x} = \frac{\partial}{\partial x}\left(\frac{x}{x^2 + y^2}\right) = \frac{(x^2 + y^2) - x(2x)}{(x^2 + y^2)^2} = \frac{x^2 + y^2 - 2x^2}{(x^2 + y^2)^2} = \frac{y^2 - x^2}{(x^2 + y^2)^2}$

Therefore:
$d\alpha = \frac{y^2 - x^2}{(x^2 + y^2)^2} dy \wedge dx + \frac{y^2 - x^2}{(x^2 + y^2)^2} dx \wedge dy$

Since $dy \wedge dx = -dx \wedge dy$:
$d\alpha = \frac{y^2 - x^2}{(x^2 + y^2)^2} (-dx \wedge dy) + \frac{y^2 - x^2}{(x^2 + y^2)^2} dx \wedge dy = 0$

% Now for the pullback under polar coordinates
$\Phi(r, \varphi) = (r\cos\varphi, r\sin\varphi)$

$x = r\cos\varphi$, $y = r\sin\varphi$
$dx = \cos\varphi dr - r\sin\varphi d\varphi$
$dy = \sin\varphi dr + r\cos\varphi d\varphi$

$\Phi^*\alpha = \frac{r\cos\varphi(sin\varphi dr + r\cos\varphi d\varphi) - r\sin\varphi(\cos\varphi dr - r\sin\varphi d\varphi)}{r^2}$

Expanding numerator:
$= r\cos\varphi\sin\varphi dr + r^2\cos^2\varphi d\varphi - r\sin\varphi\cos\varphi dr + r^2\sin^2\varphi d\varphi$
$= r^2(\cos^2\varphi + \sin^2\varphi) d\varphi$
$= r^2 d\varphi$

Therefore: $\Phi^*\alpha = d\varphi$

\end{document}