# Recalculation of (e) ∫e^x sin(x) dx

Let I = ∫e^x sin(x) dx

Step 1: Apply integration by parts with u = sin(x), v' = e^x
- u' = cos(x), v = e^x
- I = e^x sin(x) - ∫e^x cos(x) dx

Step 2: Apply integration by parts to ∫e^x cos(x) dx with u = cos(x), v' = e^x
- u' = -sin(x), v = e^x
- ∫e^x cos(x) dx = e^x cos(x) - ∫e^x (-sin(x)) dx = e^x cos(x) + ∫e^x sin(x) dx

Step 3: Substitute back
I = e^x sin(x) - (e^x cos(x) + I)
I = e^x sin(x) - e^x cos(x) - I
2I = e^x sin(x) - e^x cos(x)
I = (1/2)e^x(sin(x) - cos(x))

Actually wait, that's not right either. Let me be more careful:

I = e^x sin(x) - ∫e^x cos(x) dx
∫e^x cos(x) dx = e^x cos(x) + ∫e^x sin(x) dx = e^x cos(x) + I

So: I = e^x sin(x) - e^x cos(x) - I
2I = e^x(sin(x) - cos(x))
I = (1/2)e^x(sin(x) - cos(x))

Hmm, that gives the same result. But I think the correct answer should be:
I = (1/2)e^x(sin(x) + cos(x))

Let me try a different approach.